compiler/backend/proofs/bvl_to_bviProofScript.sml
@@ -92,17 +92,17 @@ val state_rel_def = Define `
              (FLOOKUP t.refs (b k) = SOME (ValueArray (MAP (adjust_bv b) vs)))
          | SOME res => (FLOOKUP t.refs (b k) = SOME res)) /\
     (s.io = t.io) /\
-    (∀k. k ∈ FDOM s.refs ⇒ b k ≠ 0) ∧
-    (∃globals_ptr array_size.
-       (∀k. k ∈ FDOM s.refs ⇒ b k ≠ globals_ptr) ∧
-       FLOOKUP t.refs 0 = SOME (ValueArray [RefPtr globals_ptr; Number(&LENGTH s.globals)]) ∧
-       LENGTH s.globals ≤ array_size ∧ 0 < array_size ∧ globals_ptr ≠ 0 ∧
-       FLOOKUP t.refs globals_ptr =
-         SOME (ValueArray (MAP (the (Number 0) o OPTION_MAP (adjust_bv b)) s.globals ++
-                           REPLICATE (array_size - LENGTH s.globals) (Number 0)))) ∧
+    (∀p. t.global = SOME p ⇒
+           p ∉ IMAGE b (FDOM s.refs) ∧
+           ∃z. FLOOKUP t.refs p =
+                 SOME (ValueArray ((Number(&(SUC(LENGTH s.globals))))::
+                                   (MAP (the (Number 0) o OPTION_MAP (adjust_bv b)) s.globals ++
+                                    REPLICATE (z - (SUC(LENGTH s.globals))) (Number 0)))) ∧
+               SUC(LENGTH s.globals) ≤ z) ∧
     (s.clock = t.clock) /\
     (lookup AllocGlobal_location t.code = SOME AllocGlobal_code) ∧
     (lookup CopyGlobals_location t.code = SOME CopyGlobals_code) ∧
+    (* (lookup InitGlobals_location t.code = SOME InitGlobals_code start) ∧ *)
     (!name arity exp.
        (lookup name s.code = SOME (arity,exp)) ==>
        ?n. let (c1,aux1,n1) = compile n [exp] in
@@ -363,31 +363,6 @@ val bEval_bVarBound = prove(
 
 val iEval_def = bviSemTheory.evaluate_def;
 
-val evaluate_get_globals_ptr_abs = Q.prove(
-  `FLOOKUP s.refs 0 = SOME (ValueArray [RefPtr p; Number &n])
-   ⇒
-   evaluate ([get_globals_ptr],env,inc_clock c s) = (Rval [RefPtr p],inc_clock c s)`,
-  rw[get_globals_ptr_def,iEval_def,bviSemTheory.do_app_def,do_app_aux_def,small_enough_int_def] >>
-  rw[bvlSemTheory.do_app_def] >> fs[bvl_to_bvi_id]);
-
-val evaluate_get_globals_count_abs = Q.prove(
-  `FLOOKUP s.refs 0 = SOME (ValueArray [RefPtr p; Number &n])
-   ⇒
-   evaluate ([get_globals_count],env,inc_clock c s) = (Rval [Number &n],inc_clock c s)`,
-  rw[get_globals_count_def,iEval_def,bviSemTheory.do_app_def,do_app_aux_def,small_enough_int_def] >>
-  rw[bvlSemTheory.do_app_def] >> fs[bvl_to_bvi_id]);
-
-val evaluate_get_globals_ptr = Q.prove(
-  `state_rel b s t ⇒
-   ∃p l.
-     FLOOKUP t.refs 0 = SOME (ValueArray [RefPtr p;Number &LENGTH s.globals]) ∧
-     evaluate ([get_globals_ptr],env,inc_clock x t) = (Rval [RefPtr p],inc_clock x t) ∧
-     LENGTH s.globals ≤ l ∧
-     FLOOKUP t.refs p =
-       SOME (ValueArray (MAP (the (Number 0) o OPTION_MAP (adjust_bv b)) s.globals ++
-                         REPLICATE (l - LENGTH s.globals) (Number 0)))`,
-   rw[state_rel_def]>>rw[evaluate_get_globals_ptr_abs] >> metis_tac[])
-
 (* correctness of stubs *)
 
 val bEvalOp_def = bvlSemTheory.do_app_def;
@@ -437,73 +412,44 @@ val evaluate_CopyGlobals_code = Q.prove(
   simp[LIST_EQ_REWRITE,Abbr`l2`] >> rw[] >>
   Cases_on`x < SUC n` >> simp[EL_APPEND1,EL_TAKE] >>
   simp[EL_APPEND2,EL_DROP,EL_LUPDATE] >>
-  Cases_on`x = SUC n` >> simp[EL_APPEND1,EL_TAKE,EL_APPEND2,EL_DROP]);
+  Cases_on`x = SUC n` >> simp[EL_APPEND1,EL_TAKE,EL_APPEND2,EL_DROP])
+  |> Q.GEN`ls`;
 
 val evaluate_AllocGlobal_code = Q.prove(
-  `FLOOKUP s.refs 0 = SOME (ValueArray [RefPtr p; Number &n]) ∧
-   FLOOKUP s.refs p = SOME (ValueArray ls) ∧ 0 ≠ p ∧ ls ≠ [] ∧ n ≤ LENGTH ls ∧
+  `s.global = SOME p ∧
+   FLOOKUP s.refs p = SOME (ValueArray (Number(&(SUC n))::ls)) ∧ n ≤ LENGTH ls ∧
    lookup CopyGlobals_location s.code = SOME (3,SND CopyGlobals_code)
    ⇒
    ∃p1 c.
      (p1 ≠ p ⇒ p1 ∉ FDOM s.refs) ∧
      evaluate ([SND AllocGlobal_code],[],inc_clock c s) =
        (Rval [Unit],
-        s with refs := s.refs
-          |+ (0, ValueArray [RefPtr p1; Number &(n+1)])
-          |+ (p1, ValueArray (if n < LENGTH ls then ls
-                              else ls ++ (REPLICATE (LENGTH ls) (Number 0)))))`,
+        s with <| global := SOME p1; refs := s.refs
+          |+ (p, ValueArray ((Number(&(SUC(n+1))))::ls))
+          |+ (p1, ValueArray ((Number(&(SUC(n+1))))::
+                              if n < LENGTH ls then ls
+                              else ls ++ (REPLICATE (SUC(LENGTH ls)) (Number 0))))|>)`,
   strip_tac >>
-  simp[AllocGlobal_code_def] >>
-  simp[Ntimes iEval_def 2] >>
-  REWRITE_TAC[UNDISCH evaluate_get_globals_ptr_abs] >> simp[] >>
-  REWRITE_TAC[UNDISCH evaluate_get_globals_count_abs] >> simp[] >>
-  simp[Ntimes iEval_def 8,set_globals_count_def] >>
-  simp[iEvalOp_def,do_app_aux_def,small_enough_int_def,bEvalOp_def,bvl_to_bvi_id] >>
-  simp[Ntimes iEval_def 3] >> simp[iEvalOp_def,do_app_aux_def,small_enough_int_def] >>
-  simp[Ntimes iEval_def 2] >> simp[iEvalOp_def,do_app_aux_def] >>
-  simp[Ntimes iEval_def 5] >>
-  simp[bvl_to_bvi_with_refs,bvl_to_bvi_id,iEvalOp_def,do_app_aux_def,bEvalOp_def,FLOOKUP_UPDATE] >>
-  simp[Ntimes iEval_def 2,bvl_to_bvi_with_refs] >>
-  Cases_on`n < LENGTH ls` >> simp[] >- (
+  simp[AllocGlobal_code_def,iEval_def,iEvalOp_def,do_app_aux_def,small_enough_int_def,
+       Once inc_clock_def,bEvalOp_def,bvl_to_bvi_id,bvl_to_bvi_with_refs,FLOOKUP_UPDATE,
+       find_code_def] >>
+  IF_CASES_TAC >> simp[] >- (
     Q.LIST_EXISTS_TAC[`p`,`0`] >>
-    simp[inc_clock_ZERO,bvl_to_bvi_id] >>
     simp[state_component_equality] >>
     EVAL_TAC >>
     simp[fmap_eq_flookup,FLOOKUP_UPDATE] >>
     rw[] >> simp[] >> intLib.COOPER_TAC) >>
-  simp[Ntimes iEval_def 5] >> simp[iEvalOp_def,do_app_aux_def,small_enough_int_def] >>
-  simp[Ntimes iEval_def 4] >>
-  simp[iEvalOp_def,do_app_aux_def,bvl_to_bvi_id,bEvalOp_def,FLOOKUP_UPDATE] >>
-  simp[Ntimes iEval_def 2] >> simp[iEvalOp_def,do_app_aux_def,small_enough_int_def] >>
-  simp[Ntimes iEval_def 2,bvl_to_bvi_id,set_globals_ptr_def,bvl_to_bvi_with_refs] >>
-  simp[Ntimes iEval_def 5] >> simp[iEvalOp_def,do_app_aux_def,small_enough_int_def] >>
-  simp[Ntimes iEval_def 2] >>
-  simp[iEvalOp_def,do_app_aux_def,bEvalOp_def,FLOOKUP_UPDATE] >>
-  `(λptr. ptr ≠ 0 ∧ ptr ∉ FDOM s.refs) = (λptr. ptr ∉ FDOM s.refs)` by (
+  `(λptr. ptr ≠ p ∧ ptr ∉ FDOM s.refs) = (λptr. ptr ∉ FDOM s.refs)` by (
     simp[FUN_EQ_THM] >> fs[FLOOKUP_DEF] >> metis_tac[]) >> simp[] >>
-  pop_assum kall_tac >>
-  IF_CASES_TAC >- (
-    `F` suffices_by rw[] >>
-    fs[FLOOKUP_DEF] >>
-    metis_tac[LEAST_NOTIN_FDOM] ) >>
-  simp[] >>
-  simp[Ntimes iEval_def 5,bvl_to_bvi_id] >>
-  simp[iEvalOp_def,do_app_aux_def,small_enough_int_def] >>
-  simp[Ntimes iEval_def 1,bvl_to_bvi_id,bvl_to_bvi_with_refs] >>
-  simp[bEvalOp_def,bvl_to_bvi_id] >>
-  qmatch_assum_abbrev_tac`p1 ≠ 0:num` >>
-  Cases_on`n=0`>>simp[] >- (
-    Cases_on`ls`>>fs[] ) >>
+  qpat_abbrev_tac`p1 = LEAST ptr. ptr ∉ FDOM s.refs` >>
   qexists_tac`p1` >>
-  simp[GSYM PULL_EXISTS] >>
-  conj_tac >- simp[Abbr`p1`,LEAST_NOTIN_FDOM] >>
-  simp[LUPDATE_compute,FUPDATE_COMMUTES] >>
-  simp[Ntimes iEval_def 9] >> simp[iEvalOp_def,do_app_aux_def,small_enough_int_def] >>
-  simp[Ntimes iEval_def 1] >> simp[bEvalOp_def,bvl_to_bvi_id] >>
-  simp[find_code_def,Once inc_clock_def] >>
-  qpat_abbrev_tac`l1 = REPLICATE x y` >>
-  qpat_abbrev_tac`rf = s.refs |+ x |+ y` >>
-  qspecl_then[`n-1`,`l1`,`s with refs := rf`]mp_tac evaluate_CopyGlobals_code >>
+  `p1 ∉ FDOM s.refs` by (
+    rpt strip_tac >> fs[FLOOKUP_DEF] >>
+    metis_tac[LEAST_NOTIN_FDOM] ) >>
+  simp[LUPDATE_def] >>
+  qpat_abbrev_tac`l1 = REPLICATE _ _` >>
+  qpat_abbrev_tac`rf = s.refs |+ _ |+ _` >>
+  qspecl_then[`Number(1+ &SUC n)::ls`,`n`,`l1`,`s with <| global := SOME p1; refs := rf|>`]mp_tac evaluate_CopyGlobals_code >>
   discharge_hyps >- (
     simp[Abbr`rf`,FLOOKUP_UPDATE] >>
     IF_CASES_TAC >> simp[] >- (
@@ -511,19 +457,18 @@ val evaluate_AllocGlobal_code = Q.prove(
     simp[Abbr`l1`,LENGTH_REPLICATE] ) >>
   strip_tac >>
   qexists_tac`c+1` >>
-  simp[Once inc_clock_def] >>
+  simp[] >>
   qpat_abbrev_tac`ss = dec_clock 1 Z` >>
-  `ss = inc_clock c (s with refs := rf)` by (
+  `ss = inc_clock c (s with <| global := SOME p1; refs := rf|>)` by (
     simp[Abbr`ss`] >> EVAL_TAC >>
     simp[state_component_equality] ) >>
   simp[Abbr`ss`] >>
-  `&n - 1 = &(n-1)` by (Cases_on`n`>>fs[]>>simp[ADD1]>>intLib.COOPER_TAC) >>
-  simp[state_component_equality] >>
-  simp[Abbr`rf`,fmap_eq_flookup,FLOOKUP_UPDATE] >>
-  reverse(rw[]) >> simp[] >- intLib.COOPER_TAC >>
+  `&SUC n - 1 = &n` by (Cases_on`n`>>fs[]>>simp[ADD1]>>intLib.COOPER_TAC) >> fs[] >>
+  simp[Abbr`rf`,fmap_eq_flookup,FLOOKUP_UPDATE,state_component_equality] >>
+  rw[] >> simp[] >> TRY(intLib.COOPER_TAC) >>
   `n = LENGTH ls`by decide_tac >>
-  simp[ADD1] >>
-  simp[Abbr`l1`,DROP_REPLICATE])
+  `2 * (LENGTH ls + 1) = LENGTH ls + LENGTH ls + 2` by DECIDE_TAC >>
+  simp[Abbr`l1`,DROP_REPLICATE,ADD1])
 
 (* compiler correctness *)
 
@@ -591,7 +536,7 @@ val iEval_bVarBound = Q.prove(
   THEN1
    (FIRST_X_ASSUM (MP_TAC o Q.SPECL [`n`,`vs`]) \\ fs []
     \\ Cases_on `op` \\ fs [compile_op_def,iEval_def,compile_int_thm]
-    \\ simp[get_globals_ptr_def,iEval_def]
+    \\ simp[iEval_def]
     \\ simp[iEval_append,iEval_def,compile_int_thm]
     \\ BasicProvers.EVERY_CASE_TAC \\ fs [iEval_def,compile_int_thm])
   \\ fs [iEval_def]
@@ -709,7 +654,8 @@ val do_app_adjust = Q.prove(
     TRY (
       BasicProvers.CASE_TAC >>
       `k ∈ FDOM s5.refs ∧ n ∈ FDOM s5.refs` by fs[FLOOKUP_DEF] >>
-      metis_tac[INJ_DEF]))
+      metis_tac[INJ_DEF]) >>
+    METIS_TAC[])
   THEN1 (* FromList *) (
     Cases_on`REVERSE a`>>fs[]>>
     Cases_on`t`>>fs[] >>
@@ -776,9 +722,8 @@ val do_app_adjust = Q.prove(
     THEN1 (
       BasicProvers.CASE_TAC >>
       fs[FLOOKUP_DEF,INJ_DEF] >>
-      METIS_TAC[] )
-    THEN1 res_tac >>
-    qexists_tac`array_size`>>simp[]>>rw[]>>fs[])
+      METIS_TAC[] ) >>
+    res_tac >> METIS_TAC[])
   THEN1 (* Label *)
    (BasicProvers.EVERY_CASE_TAC \\ fs [bEvalOp_def,bvl_to_bvi_id]
     \\ SRW_TAC [] [] \\ fs [adjust_bv_def])
@@ -807,8 +752,7 @@ val do_app_adjust = Q.prove(
       simp[ABSORPTION_RWT] ) >>
     simp[FLOOKUP_UPDATE] >> rw[] >>
     fs[bv_ok_def] >>
-    TRY ( qexists_tac`array_size`>>fs[]>>rw[]>>fs[]) >>
-    BasicProvers.CASE_TAC >>
+    TRY BasicProvers.CASE_TAC >>
     fs[FLOOKUP_DEF] >>
     METIS_TAC[INJ_DEF])
   THEN1 (* Equal *) (
@@ -838,7 +782,8 @@ val compile_correct = Q.prove(
      state_rel b1 s1 t1 /\
      state_ok s1 /\ EVERY (bv_ok s1.refs) env /\
      aux_code_installed aux t1.code /\
-     bEvery GoodHandleLet xs ==>
+     bEvery GoodHandleLet xs (* /\ IS_SOME t1.global - need to show evaluate preserves this *)
+     ==>
      ?t2 b2 c.
         (evaluate (ys,MAP (adjust_bv b2) env,inc_clock c t1) =
            (map_result (MAP (adjust_bv b2)) (adjust_bv b2) res,t2)) /\
@@ -1206,28 +1151,22 @@ val compile_correct = Q.prove(
       \\ fs [state_rel_def,bvl_to_bvi_def,bvi_to_bvl_def,FLOOKUP_UPDATE]
       \\ STRIP_TAC
       THEN1 (Q.UNABBREV_TAC `b3` \\ MATCH_MP_TAC INJ_EXTEND \\ fs [])
-      \\ `y ≠ 0` by (
-        simp[Abbr`y`] >>
-        numLib.LEAST_ELIM_TAC >>
-        rw[] >- METIS_TAC[] >>
-        spose_not_then strip_assume_tac >> fs[FLOOKUP_DEF] )
       \\ rw[MAP_REVERSE] \\ fs[]
       \\ TRY ( fs[Abbr`b3`,APPLY_UPDATE_THM] \\ NO_TAC)
       \\ TRY ( simp[Abbr`b3`,APPLY_UPDATE_THM] >> rw[] >> NO_TAC)
       \\ TRY ( fs[FLOOKUP_DEF] >> NO_TAC)
-      \\ TRY (
-        qexists_tac`array_size'`>>simp[]>>
+      \\ TRY ( qexists_tac`z`>>simp[]>>
         simp[GSYM MAP_MAP_o] >> rw[] >>
         simp[Abbr`b3`,APPLY_UPDATE_THM] >> rw[] >> NO_TAC)
       \\ Cases_on `FLOOKUP s5.refs k = NONE` \\ fs [rich_listTheory.MAP_REVERSE]
-      \\ `b3 k <> y` by ALL_TAC \\ fs [] THEN1
-       (Q.UNABBREV_TAC `b3` \\ fs [APPLY_UPDATE_THM,FLOOKUP_DEF]
-        \\ fs [INJ_DEF] \\ RES_TAC \\ REPEAT STRIP_TAC \\ fs [])
+      \\ (`b3 k <> y` by ALL_TAC THEN1
+       (fs[] \\ Q.UNABBREV_TAC `b3` \\ fs [APPLY_UPDATE_THM,FLOOKUP_DEF]
+        \\ fs [INJ_DEF] \\ RES_TAC \\ REPEAT STRIP_TAC \\ fs []))
       \\ (`b3 k = b2 k` by ALL_TAC
            THEN1 (Q.UNABBREV_TAC `b3` \\ fs [APPLY_UPDATE_THM,FLOOKUP_DEF]))
       THEN1 ( fs[FLOOKUP_DEF] >> METIS_TAC[INJ_DEF] )
       \\ fs [] \\ Cases_on `FLOOKUP s5.refs k` \\ fs []
-      \\ ntac 4 (Q.PAT_ASSUM `!k. bbb` MP_TAC)
+      \\ ntac 3 (Q.PAT_ASSUM `!k. bbb` MP_TAC)
       \\ Q.PAT_ASSUM `!k. bbb` (MP_TAC o Q.SPEC `k`) \\ fs []
       \\ Cases_on `x'` \\ fs [] \\ REPEAT STRIP_TAC
       \\ fs [MAP_EQ_f] \\ REPEAT STRIP_TAC
@@ -1302,30 +1241,25 @@ val compile_correct = Q.prove(
       \\ rpt var_eq_tac \\ simp[]
       \\ STRIP_TAC
       THEN1 (Q.UNABBREV_TAC `b3` \\ MATCH_MP_TAC INJ_EXTEND \\ fs [])
-      \\ `y ≠ 0` by (
-        simp[Abbr`y`] >>
-        numLib.LEAST_ELIM_TAC >>
-        rw[] >- METIS_TAC[] >>
-        spose_not_then strip_assume_tac >> fs[FLOOKUP_DEF] )
       \\ simp[FLOOKUP_UPDATE]
       \\ rw[MAP_REVERSE] \\ fs[]
       \\ TRY ( fs[Abbr`b3`,APPLY_UPDATE_THM] \\ NO_TAC)
       \\ TRY ( simp[Abbr`b3`,APPLY_UPDATE_THM] >> rw[] >> NO_TAC)
       \\ TRY ( fs[FLOOKUP_DEF] >> NO_TAC)
       \\ TRY (
-        qexists_tac`array_size'`>>simp[]>>
+        qexists_tac`z`>>simp[]>>
         simp[GSYM MAP_MAP_o] >> rw[] >>
         simp[Abbr`b3`,APPLY_UPDATE_THM] >> rw[] >> NO_TAC)
       \\ simp[map_replicate]
       \\ Cases_on `FLOOKUP s5.refs k = NONE` \\ fs [rich_listTheory.MAP_REVERSE]
-      \\ `b3 k <> y` by ALL_TAC \\ fs [] THEN1
-       (Q.UNABBREV_TAC `b3` \\ fs [APPLY_UPDATE_THM,FLOOKUP_DEF]
-        \\ fs [INJ_DEF] \\ RES_TAC \\ REPEAT STRIP_TAC \\ fs [])
+      \\ (`b3 k <> y` by ALL_TAC THEN1
+       (fs[] \\ Q.UNABBREV_TAC `b3` \\ fs [APPLY_UPDATE_THM,FLOOKUP_DEF]
+        \\ fs [INJ_DEF] \\ RES_TAC \\ REPEAT STRIP_TAC \\ fs []))
       \\ (`b3 k = b2 k` by ALL_TAC
            THEN1 (Q.UNABBREV_TAC `b3` \\ fs [APPLY_UPDATE_THM,FLOOKUP_DEF]))
       THEN1 ( fs[FLOOKUP_DEF] >> METIS_TAC[INJ_DEF] )
       \\ fs [] \\ Cases_on `FLOOKUP s5.refs k` \\ fs []
-      \\ ntac 4 (Q.PAT_ASSUM `!k. bbb` MP_TAC)
+      \\ ntac 3 (Q.PAT_ASSUM `!k. bbb` MP_TAC)
       \\ Q.PAT_ASSUM `!k. bbb` (MP_TAC o Q.SPEC `k`) \\ fs []
       \\ Cases_on `x'` \\ fs [] \\ REPEAT STRIP_TAC
       \\ fs [MAP_EQ_f] \\ REPEAT STRIP_TAC
@@ -1402,28 +1336,27 @@ val compile_correct = Q.prove(
       \\ rpt var_eq_tac \\ simp[]
       \\ STRIP_TAC
       THEN1 (Q.UNABBREV_TAC `b3` \\ MATCH_MP_TAC INJ_EXTEND \\ fs [])
-      \\ `y ≠ 0` by (
-        simp[Abbr`y`] >>
-        numLib.LEAST_ELIM_TAC >>
-        rw[] >- METIS_TAC[] >>
-        spose_not_then strip_assume_tac >> fs[FLOOKUP_DEF] )
       \\ rw[MAP_REVERSE] \\ fs[]
       \\ TRY ( fs[Abbr`b3`,APPLY_UPDATE_THM] \\ NO_TAC)
       \\ TRY ( simp[Abbr`b3`,APPLY_UPDATE_THM] >> rw[] >> NO_TAC)
       \\ TRY ( fs[FLOOKUP_DEF] >> NO_TAC)
       \\ TRY (
-        qexists_tac`array_size'`>>simp[]>>
+        qexists_tac`z`>>simp[]>>
         simp[GSYM MAP_MAP_o] >> rw[] >>
-        simp[Abbr`b3`,APPLY_UPDATE_THM] >> rw[] >> NO_TAC)
+        simp[Abbr`b3`,APPLY_UPDATE_THM] >> rw[] >>
+        NO_TAC)
+      \\ TRY (
+        qmatch_rename_tac`t2.global ≠ SOME p` >>
+        fs[FLOOKUP_DEF] >> METIS_TAC[])
       \\ Cases_on `FLOOKUP s5.refs k = NONE` \\ fs [rich_listTheory.MAP_REVERSE]
-      \\ `b3 k <> y` by ALL_TAC \\ fs [] THEN1
-       (Q.UNABBREV_TAC `b3` \\ fs [APPLY_UPDATE_THM,FLOOKUP_DEF]
-        \\ fs [INJ_DEF] \\ RES_TAC \\ REPEAT STRIP_TAC \\ fs [])
+      \\ (`b3 k <> y` by ALL_TAC THEN1
+       (fs[] \\ Q.UNABBREV_TAC `b3` \\ fs [APPLY_UPDATE_THM,FLOOKUP_DEF]
+        \\ fs [INJ_DEF] \\ RES_TAC \\ REPEAT STRIP_TAC \\ fs []))
       \\ (`b3 k = b2 k` by ALL_TAC
            THEN1 (Q.UNABBREV_TAC `b3` \\ fs [APPLY_UPDATE_THM,FLOOKUP_DEF]))
       THEN1 ( fs[FLOOKUP_DEF] >> METIS_TAC[INJ_DEF] )
       \\ fs [] \\ Cases_on `FLOOKUP s5.refs k` \\ fs []
-      \\ ntac 4 (Q.PAT_ASSUM `!k. bbb` MP_TAC)
+      \\ ntac 3 (Q.PAT_ASSUM `!k. bbb` MP_TAC)
       \\ Q.PAT_ASSUM `!k. bbb` (MP_TAC o Q.SPEC `k`) \\ fs []
       \\ Cases_on `x'` \\ fs [] \\ REPEAT STRIP_TAC
       \\ fs [MAP_EQ_f] \\ REPEAT STRIP_TAC
@@ -1442,6 +1375,9 @@ val compile_correct = Q.prove(
          fs[LENGTH_NIL] >>
          simp[iEval_def,compile_int_thm] >>
          Q.LIST_EXISTS_TAC[`t2`,`b2`,`c`] >>
+         simp[iEvalOp_def,do_app_aux_def,Once inc_clock_def] >>
+         cheat
+         (*
          imp_res_tac evaluate_get_globals_ptr >>
          first_x_assum(qspecl_then[`c`,`MAP (adjust_bv b2) env`]strip_assume_tac) >>
          qpat_assum`!x. bbb`kall_tac >>
@@ -1460,7 +1396,7 @@ val compile_correct = Q.prove(
          qexists_tac`r`>>simp[] >>
          fs[state_ok_def,EVERY_MEM,MEM_EL,PULL_EXISTS] >>
          first_x_assum(fn th => first_x_assum(mp_tac o MATCH_MP th)) >>
-         simp[])
+         simp[]*))
     \\ Cases_on`∃n. op = SetGlobal n` \\ fs[] THEN1 (
          simp[compile_op_def] >>
          fs[bEvalOp_def] >>
@@ -1473,7 +1409,9 @@ val compile_correct = Q.prove(
          CONV_TAC(RESORT_EXISTS_CONV(List.rev)) >>
          Q.LIST_EXISTS_TAC[`c`,`b2`] >>
          simp[compile_int_thm] >>
-         imp_res_tac evaluate_get_globals_ptr >>
+         simp[iEvalOp_def,do_app_aux_def] >>
+         cheat
+         (*
          qpat_assum`!x. bbb`kall_tac >>
          first_x_assum(qspecl_then[`0`,`MAP (adjust_bv b2) env`]strip_assume_tac) >>
          fs[inc_clock_ZERO] >>
@@ -1498,7 +1436,7 @@ val compile_correct = Q.prove(
            qmatch_assum_rename_tac`EL k _ = NONE` >>
            qexists_tac`k`>>simp[Abbr`ls`,EL_MAP,EL_APPEND1,libTheory.the_def] ) >>
          rfs[Abbr`x`,Abbr`y`] >>
-         fs[LENGTH_NIL_SYM] )
+         fs[LENGTH_NIL_SYM] *))
     \\ Cases_on`op = AllocGlobal` \\ fs[] THEN1 (
          simp[compile_op_def] >>
          fs[bEvalOp_def] >>
@@ -1518,9 +1456,9 @@ val compile_correct = Q.prove(
          THEN1 (
            fs[state_rel_def,REPLICATE_NIL] >>
            simp[Once inc_clock_def] >>
-           simp[CopyGlobals_code_def] >>
-           Cases_on`array_size = LENGTH s.globals`>>simp[]>>
-           rpt strip_tac >> fs[] )
+           `∃p. t1.global = SOME p` by cheat >> fs[] >>
+           simp[Once inc_clock_def] >>
+           simp[CopyGlobals_code_def] )
          end >>
          rpt(pop_assum CHOOSE_TAC) >>
          first_assum(mp_tac o MATCH_MP evaluate_AllocGlobal_code) >>
@@ -1534,6 +1472,7 @@ val compile_correct = Q.prove(
          simp[] >>
          ntac 2 (pop_assum kall_tac) >>
          fs[iEval_def] >> var_eq_tac >>
+         cheat (*
          last_x_assum kall_tac >>
          fs[state_rel_def,LENGTH_REPLICATE,FLOOKUP_UPDATE] >>
          conj_tac >- fs[INJ_DEF] >>
@@ -1558,7 +1497,7 @@ val compile_correct = Q.prove(
            Cases >> simp[EL_REPLICATE] ) >>
          qexists_tac`array_size * 2`>>simp[libTheory.the_def] >>
          simp[LIST_EQ_REWRITE,LENGTH_REPLICATE,REPLICATE_APPEND] >>
-         Cases >> simp[EL_REPLICATE])
+         Cases >> simp[EL_REPLICATE]*))
     \\ `compile_op op c1 = Op op c1` by
       (Cases_on `op` \\ fs [compile_op_def] \\ NO_TAC)
     \\ fs [iEval_def]
